Refactor: use Base and unify notations for module names.
Also fixed errors due to implicit argument declarations in Base.

Structure.v
@@ -1,16 +1,10 @@
-Require Coq.Unicode.Utf8.
-Require Coq.Vectors.Vector.
-Require Import Arith Bool.
-Require Import FunctionalExtensionality.
-Require Import Sets.Ensembles.
-Require Import CFOLID.Signature.
-Require Import CFOLID.Term.
+Require Import Base Signature Term.
 
 Section structure.
   Variable Σ : signature.
 
-  Structure structure := {      (* struktura *)
-      domain : Type;            (* nosač *)
+  Structure structure := {
+      domain : Type;
       interpF : forall f : FuncS Σ, vec domain (FuncArr f) -> domain;
       interpP : forall P : PredS Σ, vec domain (PredArr P) -> Prop;
       interpIP : forall P : IndPredS Σ, vec domain (IndPredArr P) -> Prop;
@@ -39,16 +33,16 @@ Section environment.
     Fixpoint env (t : term Σ) : |M| :=
       match t with
       | TVar x => ρvar x
-      | TFunc f args => interpF M f (Vector.map env args)
+      | TFunc f args => interpF M f (V.map env args)
       end.
 
     Definition env_vec n (v : vec (term Σ) n) : vec (|M|) n :=
-      Vector.map env v.
+      V.map env v.
 
     Fixpoint env_subst (t : term Σ) (x : var) (d : |M|) : |M| :=
       match t with
       | TVar y => env_var_subst ρvar x d y
-      | TFunc f args => interpF M f (Vector.map (fun st => env_subst st x d) args)
+      | TFunc f args => interpF M f (V.map (fun st => env_subst st x d) args)
       end.
   End extended_environment.
 
@@ -59,7 +53,7 @@ Section environment.
     Variable x : var.
 
     Lemma env_subst_sanity1 : forall (d : |M|),
-        ~ In _ (Var t) x -> env_subst ρvar t x d = env ρvar t.
+        ~ E.In (Var t) x -> env_subst ρvar t x d = env ρvar t.
     Proof.
       induction t as [v | f args IH] using term_better_ind;
         intros d x_not_in_t.
@@ -67,12 +61,12 @@ Section environment.
         + exfalso. apply x_not_in_t. rewrite Nat.eqb_eq in eq_vx; subst.
           constructor.
         + reflexivity.
-      - simpl. f_equal. apply Vector.map_ext_in.
-        intros st Hin. rewrite Vector.Forall_forall in IH.
+      - simpl. f_equal. apply V.map_ext_in.
+        intros st Hin. rewrite V.Forall_forall in IH.
         apply IH.
         + assumption.
         + intros x_in_var_st. apply x_not_in_t.
-          constructor. apply vec_In_Ex with st; assumption.
+          constructor. apply Exists_exists; exists st; intuition.
     Qed. 
 
     Lemma env_subst_sanity2 : forall (u : term Σ),
@@ -81,8 +75,8 @@ Section environment.
       intros u. induction t as [v | f args IH] using term_better_ind2.
       - cbn. unfold env_var_subst. destruct (v =? x) eqn:E;
           reflexivity.
-      - simpl. f_equal. rewrite Vector.map_map.
-        apply Vector.map_ext_in. intros st Hst.
+      - simpl. f_equal. rewrite V.map_map.
+        apply V.map_ext_in. intros st Hst.
         apply IH. assumption.
     Qed.
       
