Term.v
@@ -1,10 +1,5 @@
-Require Import Coq.Unicode.Utf8.
-Require Import Coq.Vectors.Vector.
-Require Import Coq.Sets.Ensembles.
-Require Import CFOLID.Signature.
-Require Import Arith.
-
-Definition vec := Vector.t.
+Require Import Base.
+Require Import Signature.
 
 Section term.
   Variable Σ : signature.
@@ -21,7 +16,7 @@ Section term.
     
     Hypothesis Pbase : forall v, P (TVar v).
     Hypothesis Pind : forall (f : FuncS Σ) (args : vec term (FuncArr f)),
-        Vector.Forall (fun st => P st) args -> P (TFunc f args).
+        V.Forall (fun st => P st) args -> P (TFunc f args).
     
     Definition term_better_ind : forall t : term, P t.
       fix IND_PRINCIPLE 1; intros [v | f args].
@@ -36,12 +31,12 @@ Section term.
     Variable P : term -> Prop.
     Hypothesis Pbase : forall v, P (TVar v).
     Hypothesis Pind : forall (f : FuncS Σ) (args : vec term (FuncArr f)),
-        (forall st : term, Vector.In st args -> P st) -> P (TFunc f args).
+        (forall st : term, V.In st args -> P st) -> P (TFunc f args).
 
     Definition term_better_ind2 : forall t : term, P t.
       induction t as [v | f args IH] using term_better_ind.
       - apply Pbase.
-      - apply Pind. intros st Hin. rewrite Forall_forall in IH.
+      - apply Pind. intros st Hin. rewrite V.Forall_forall in IH.
         apply IH. apply Hin.
     Defined.
   End term_better_ind2.    
@@ -51,14 +46,14 @@ Section term.
   Fixpoint term_var_subst (t : term) (u : term) (x : var) : term :=
     match t with
     | TVar v => if v =? x then u else t
-    | TFunc f args => TFunc f (map (fun st => term_var_subst st u x) args)
+    | TFunc f args => TFunc f (V.map (fun st => term_var_subst st u x) args)
     end.
 
   (* The set of all variables of a given term. *)
-  Inductive Var : term -> Ensemble var :=
+  Inductive Var : term -> E.Ensemble var :=
   | VarVar : forall (v : var), Var (TVar v) v
   | VarFunc : forall (f : FuncS Σ) (args : vec term (FuncArr f)) (v : var),
-      Exists (fun t => Var t v) args -> Var (TFunc f args) v.
+      V.Exists (fun t => Var t v) args -> Var (TFunc f args) v.
 End term.
 
 Arguments TVar {Σ} _.
@@ -76,28 +71,19 @@ Section term_facts.
   Open Scope term_scope.
   Variable Σ : signature.
 
-  Lemma var_not_in_Var_not_eq : forall v x, ~ In _ (@Var Σ( TVar v)) x -> v <> x.
+  Lemma var_not_in_Var_not_eq : forall v x, ~ E.In (@Var Σ (TVar v)) x -> v <> x.
   Proof.
     intros v x H. intros eq. apply H. subst; constructor.
-  Qed.
-
-  Lemma vec_In_Ex : forall (A : Type) (n : nat) (v : vec A n) (a : A) (P : A -> Prop),
-      Vector.In a v -> P a -> Exists (fun e => P e) v.
-  Proof.
-    intros A n v a P Hin HP. induction v.
-    - inversion Hin.
-    - apply In_cons_iff in Hin; destruct Hin as [Hhead | Hcons].
-      + apply Exists_cons_hd. rewrite Hhead. apply HP.
-      + apply Exists_cons_tl. intuition.
   Qed.
   
   Lemma var_not_in_Func_not_in_args :
     forall (f : FuncS Σ) (args : vec (term Σ) (FuncArr f)) (x : var),
-      ~ In _ (Var (TFunc f args)) x -> Vector.Forall (fun st => ~ In _ (Var st) x) args.
+      ~ E.In (Var (TFunc f args)) x -> V.Forall (fun st => ~ E.In (Var st) x) args.
   Proof.
-    intros f args x Hnotin; rewrite Forall_forall; unfold In in *.
+    intros f args x Hnotin; rewrite V.Forall_forall; unfold E.In in *.
     intros t Hin Hvar. apply Hnotin. constructor.
-    apply vec_In_Ex with t; assumption.
+    apply Exists_exists.
+    exists t; intuition.
   Qed.
     
   Lemma term_var_subst_id : forall (t : term Σ) (x : var),
@@ -115,17 +101,17 @@ Section term_facts.
   Qed.
     
   Lemma term_var_subst_no_occ : forall (t u : term Σ) (x : var),
-      ~ In _ (Var t) x -> t [x => u] = t.
+      ~ E.In (Var t) x -> t [x => u] = t.
   Proof.
     intros t; induction t as [v | f args IH] using term_better_ind2;
       intros u x Hnotin; cbn.
     - destruct (v =? x) eqn:E.
       + exfalso; apply Hnotin; rewrite Nat.eqb_eq in E; subst; constructor.
       + reflexivity.
-    - f_equal. rewrite <- map_id. apply map_ext_in.
+    - f_equal. rewrite <- V.map_id. apply V.map_ext_in.
       intros st Hstin. apply IH.
       + assumption.
-      + intros Hinvar.
-        apply Hnotin. constructor. apply vec_In_Ex with st; assumption.
+      + intros Hinvar. apply Hnotin. constructor.
+        apply Exists_exists. exists st; intuition.
   Qed.
 End term_facts.
