CFOLID.v
@@ -1,3 +1,4 @@
+Require Export CFOLID.Base.
 Require Export CFOLID.Signature.
 Require Export CFOLID.Term.
 Require Export CFOLID.Formula.
